Change the model for higher-order values not to support the construction of composite values over program values. Also enhanced sorts by incorporating value refinement into a new sort VALUE_SORT. Inverse functions have been removed from the sorts to facilitate instantiation of HO1 and HO2 values. Finally, I made changes to the parametrisation of type synonyms in various places and added a designated theory utp_types.thy for them. There has been minor polishing in a few other places.

theories/GLOBAL.thy
@@ -3,159 +3,145 @@
 (* Author: Frank Zeyda, University of York                                    *)
 (******************************************************************************)
 theory GLOBAL
-imports "utp_common" "generic/utp_name"
+imports utp_common utp_types
 begin
-
-section {* Type Synonyms *}
-
-types 'TYPE VAR = "NAME \<times> 'TYPE"
-types 'VAR ALPHABET = "'VAR set"
-types ('VAR, 'VALUE) BINDING = "'VAR \<Rightarrow> 'VALUE"
-types ('VAR, 'VALUE) BINDING_SET = "('VAR, 'VALUE) BINDING set"
-types ('VAR, 'VALUE) BINDING_FUN = "('VAR, 'VALUE) BINDING \<Rightarrow> bool"
-types ('VAR, 'VALUE) ALPHA_PREDICATE =
-  "('VAR ALPHABET) \<times> ('VAR, 'VALUE) BINDING_SET"
-
-types ('VAR, 'VALUE) ALPHA_FUNCTION =
-  "('VAR, 'VALUE) ALPHA_PREDICATE \<Rightarrow>
-   ('VAR, 'VALUE) ALPHA_PREDICATE"
 
 section {* Global Syntax *}
 
 subsection {* Value Syntax *}
 
 consts type_rel :: "'VALUE \<Rightarrow> 'TYPE \<Rightarrow> bool" (infix ":" 50)
+
 consts set_type_rel :: "'VALUE set \<Rightarrow> 'TYPE \<Rightarrow> bool" (infix ":\<subseteq>" 50)
-consts value_ref :: "'VALUE \<Rightarrow> 'VALUE \<Rightarrow> bool" (infix "\<sqsubseteq>v" 50)
 
 subsection {* Predicate Syntax *}
 
 consts alphabet ::
-  "('VAR, 'VALUE) ALPHA_PREDICATE \<Rightarrow>
-   ('VAR ALPHABET)" ("\<alpha>")
+  "('VALUE, 'TYPE) ALPHA_PREDICATE \<Rightarrow>
+   ('TYPE ALPHABET)" ("\<alpha>")
 
 consts bindings ::
-  "('VAR, 'VALUE) ALPHA_PREDICATE \<Rightarrow>
-   ('VAR, 'VALUE) BINDING_SET" ("\<beta>")
+  "('VALUE, 'TYPE) ALPHA_PREDICATE \<Rightarrow>
+   ('VALUE, 'TYPE) BINDING_SET" ("\<beta>")
 
-consts BINDING_EQUIV ::
-  "('VAR, 'VALUE) BINDING \<Rightarrow>
-   ('VAR, 'VALUE) BINDING \<Rightarrow>
-   ('VAR ALPHABET) \<Rightarrow> bool"
+consts binding_equiv ::
+  "('VALUE, 'TYPE) BINDING \<Rightarrow>
+   ('VALUE, 'TYPE) BINDING \<Rightarrow>
+   ('TYPE ALPHABET) \<Rightarrow> bool"
   ("_ \<cong> _ on _")
 
 consts LiftP ::
-  "('VAR ALPHABET) \<Rightarrow>
-   (('VAR, 'VALUE) BINDING_FUN) \<Rightarrow>
-   ('VAR, 'VALUE) ALPHA_PREDICATE"
+  "('TYPE ALPHABET) \<Rightarrow>
+   ('VALUE, 'TYPE) BINDING_FUN \<Rightarrow>
+   ('VALUE, 'TYPE) ALPHA_PREDICATE"
 
 syntax "LiftP_Syntax" ::
-  "'VAR ALPHABET \<Rightarrow> idt \<Rightarrow> bool \<Rightarrow>
-   ('VAR, 'VALUE) ALPHA_PREDICATE" ("(1_ \<odot> _ \<bullet>/ _)")
+  "'TYPE ALPHABET \<Rightarrow> idt \<Rightarrow> bool \<Rightarrow>
+   ('VALUE, 'TYPE) ALPHA_PREDICATE" ("(1_ \<odot> _ \<bullet>/ _)")
 
 translations
   "a \<odot> b \<bullet> P" == "CONST LiftP a (\<lambda> b . P)"
 
 consts TrueP ::
-  "'VAR ALPHABET \<Rightarrow> ('VAR, 'VALUE) ALPHA_PREDICATE" ("true")
+  "'TYPE ALPHABET \<Rightarrow> ('VALUE, 'TYPE) ALPHA_PREDICATE" ("true")
 
 consts FalseP ::
-  "'VAR ALPHABET \<Rightarrow> ('VAR, 'VALUE) ALPHA_PREDICATE" ("false")
+  "'TYPE ALPHABET \<Rightarrow> ('VALUE, 'TYPE) ALPHA_PREDICATE" ("false")
 
 consts TRUE ::
-  "('VAR, 'VALUE) ALPHA_PREDICATE" ("TRUE")
+  "('VALUE, 'TYPE) ALPHA_PREDICATE" ("TRUE")
 
 consts FALSE ::
-  "('VAR, 'VALUE) ALPHA_PREDICATE" ("FALSE")
+  "('VALUE, 'TYPE) ALPHA_PREDICATE" ("FALSE")
 
 consts ExtP ::
-  "('VAR, 'VALUE) ALPHA_PREDICATE \<Rightarrow> 'VAR ALPHABET \<Rightarrow>
-   ('VAR, 'VALUE) ALPHA_PREDICATE"
+  "('VALUE, 'TYPE) ALPHA_PREDICATE \<Rightarrow> 'TYPE ALPHABET \<Rightarrow>
+   ('VALUE, 'TYPE) ALPHA_PREDICATE"
   (infix "\<oplus>" 200)
 
 consts ResP ::
-  "('VAR, 'VALUE) ALPHA_PREDICATE \<Rightarrow> 'VAR ALPHABET \<Rightarrow>
-   ('VAR, 'VALUE) ALPHA_PREDICATE"
+  "('VALUE, 'TYPE) ALPHA_PREDICATE \<Rightarrow> 'TYPE ALPHABET \<Rightarrow>
+   ('VALUE, 'TYPE) ALPHA_PREDICATE"
   (infix "\<ominus>" 200)
 
 consts NotP ::
-  "('VAR, 'VALUE) ALPHA_PREDICATE \<Rightarrow>
-   ('VAR, 'VALUE) ALPHA_PREDICATE"
+  "('VALUE, 'TYPE) ALPHA_PREDICATE \<Rightarrow>
+   ('VALUE, 'TYPE) ALPHA_PREDICATE"
   ("\<not>p _" [190] 190)
 
 consts AndP ::
-  "('VAR, 'VALUE) ALPHA_PREDICATE \<Rightarrow>
-   ('VAR, 'VALUE) ALPHA_PREDICATE \<Rightarrow>
-   ('VAR, 'VALUE) ALPHA_PREDICATE"
+  "('VALUE, 'TYPE) ALPHA_PREDICATE \<Rightarrow>
+   ('VALUE, 'TYPE) ALPHA_PREDICATE \<Rightarrow>
+   ('VALUE, 'TYPE) ALPHA_PREDICATE"
   (infixr "\<and>p" 180)
 
 consts OrP ::
-  "('VAR, 'VALUE) ALPHA_PREDICATE \<Rightarrow>
-   ('VAR, 'VALUE) ALPHA_PREDICATE \<Rightarrow>
-   ('VAR, 'VALUE) ALPHA_PREDICATE"
+  "('VALUE, 'TYPE) ALPHA_PREDICATE \<Rightarrow>
+   ('VALUE, 'TYPE) ALPHA_PREDICATE \<Rightarrow>
+   ('VALUE, 'TYPE) ALPHA_PREDICATE"
   (infixr "\<or>p" 170)
 
 consts ImpliesP ::
-  "('VAR, 'VALUE) ALPHA_PREDICATE \<Rightarrow>
-   ('VAR, 'VALUE) ALPHA_PREDICATE \<Rightarrow>
-   ('VAR, 'VALUE) ALPHA_PREDICATE"
+  "('VALUE, 'TYPE) ALPHA_PREDICATE \<Rightarrow>
+   ('VALUE, 'TYPE) ALPHA_PREDICATE \<Rightarrow>
+   ('VALUE, 'TYPE) ALPHA_PREDICATE"
   (infixr "\<Rightarrow>p" 160)
 
 consts IffP ::
-  "('VAR, 'VALUE) ALPHA_PREDICATE \<Rightarrow>
-   ('VAR, 'VALUE) ALPHA_PREDICATE \<Rightarrow>
-   ('VAR, 'VALUE) ALPHA_PREDICATE"
+  "('VALUE, 'TYPE) ALPHA_PREDICATE \<Rightarrow>
+   ('VALUE, 'TYPE) ALPHA_PREDICATE \<Rightarrow>
+   ('VALUE, 'TYPE) ALPHA_PREDICATE"
   (infixr "\<Leftrightarrow>p" 150)
 
 consts ExistsResP ::
-  "('VAR ALPHABET) \<Rightarrow>
-   ('VAR, 'VALUE) ALPHA_PREDICATE \<Rightarrow>
-   ('VAR, 'VALUE) ALPHA_PREDICATE"
+  "('TYPE ALPHABET) \<Rightarrow>
+   ('VALUE, 'TYPE) ALPHA_PREDICATE \<Rightarrow>
+   ('VALUE, 'TYPE) ALPHA_PREDICATE"
   ("(\<exists>-p _ ./ _)" [0, 10] 10)
 
 consts ForallResP ::
-  "('VAR ALPHABET) \<Rightarrow>
-   ('VAR, 'VALUE) ALPHA_PREDICATE \<Rightarrow>
-   ('VAR, 'VALUE) ALPHA_PREDICATE"
+  "('TYPE ALPHABET) \<Rightarrow>
+   ('VALUE, 'TYPE) ALPHA_PREDICATE \<Rightarrow>
+   ('VALUE, 'TYPE) ALPHA_PREDICATE"
   ("(\<forall>-p _ ./ _)" [0, 10] 10)
 
 consts ExistsP ::
-  "('VAR ALPHABET) \<Rightarrow>
-   ('VAR, 'VALUE) ALPHA_PREDICATE \<Rightarrow>
-   ('VAR, 'VALUE) ALPHA_PREDICATE"
+  "('TYPE ALPHABET) \<Rightarrow>
+   ('VALUE, 'TYPE) ALPHA_PREDICATE \<Rightarrow>
+   ('VALUE, 'TYPE) ALPHA_PREDICATE"
   ("(\<exists>p _ ./ _)" [0, 10] 10)
 
 consts ForallP ::
-  "('VAR ALPHABET) \<Rightarrow>
-   ('VAR, 'VALUE) ALPHA_PREDICATE \<Rightarrow>
-   ('VAR, 'VALUE) ALPHA_PREDICATE"
+  "('TYPE ALPHABET) \<Rightarrow>
+   ('VALUE, 'TYPE) ALPHA_PREDICATE \<Rightarrow>
+   ('VALUE, 'TYPE) ALPHA_PREDICATE"
   ("(\<forall>p _ ./ _)" [0, 10] 10)
 
 consts ClosureP ::
-  "('VAR, 'VALUE) ALPHA_PREDICATE \<Rightarrow>
-   ('VAR, 'VALUE) ALPHA_PREDICATE"
+  "('VALUE, 'TYPE) ALPHA_PREDICATE \<Rightarrow>
+   ('VALUE, 'TYPE) ALPHA_PREDICATE"
   ("[_]")
 
 consts RefP ::
-  "('VAR, 'VALUE) ALPHA_PREDICATE \<Rightarrow>
-   ('VAR, 'VALUE) ALPHA_PREDICATE \<Rightarrow>
-   ('VAR, 'VALUE) ALPHA_PREDICATE"
+  "('VALUE, 'TYPE) ALPHA_PREDICATE \<Rightarrow>
+   ('VALUE, 'TYPE) ALPHA_PREDICATE \<Rightarrow>
+   ('VALUE, 'TYPE) ALPHA_PREDICATE"
   (infix "\<sqsubseteq>p" 100)
 
 consts Tautology ::
-  "('VAR, 'VALUE) ALPHA_PREDICATE \<Rightarrow> bool"
+  "('VALUE, 'TYPE) ALPHA_PREDICATE \<Rightarrow> bool"
   ("taut _" [50] 50)
 
 consts Contradiction ::
-  "('VAR, 'VALUE) ALPHA_PREDICATE \<Rightarrow> bool"
+  "('VALUE, 'TYPE) ALPHA_PREDICATE \<Rightarrow> bool"
   ("contra _" [50] 50)
 
 consts Contingency ::
-  "('VAR, 'VALUE) ALPHA_PREDICATE \<Rightarrow> bool"
+  "('VALUE, 'TYPE) ALPHA_PREDICATE \<Rightarrow> bool"
   ("contg _" [50] 50)
 
 consts Refinement ::
-  "('VAR, 'VALUE) ALPHA_PREDICATE \<Rightarrow>
-   ('VAR, 'VALUE) ALPHA_PREDICATE \<Rightarrow> bool"
+  "('VALUE, 'TYPE) ALPHA_PREDICATE \<Rightarrow>
+   ('VALUE, 'TYPE) ALPHA_PREDICATE \<Rightarrow> bool"
   (infix "\<sqsubseteq>" 50)
 end
