theories/generic/utp_composite_value.thy
@@ -8,12 +8,9 @@ begin
 
 section {* Composite Values *}
 
-subsection {* Data Types *}
+subsection {* Value Encoding *}
 
-text {*
-  The @{text "SetVal"} constructor might need to know about the type of
-  elements the set.
-*}
+text {* Does @{text "SetVal"} need to know about the type of the set? *}
 
 datatype 'BASIC_VALUE COMPOSITE_VALUE =
   BasicVal "'BASIC_VALUE" |
@@ -27,9 +24,9 @@ datatype 'BASIC_TYPE COMPOSITE_TYPE =
 
 subsubsection {* Destructors *}
 
-primrec ValOf ::
+primrec BasicOf ::
   "'BASIC_VALUE COMPOSITE_VALUE \<Rightarrow> 'BASIC_VALUE" where
-"ValOf (BasicVal v) = v"
+"BasicOf (BasicVal v) = v"
 
 primrec PairOf ::
   "'BASIC_VALUE COMPOSITE_VALUE \<Rightarrow>
@@ -74,89 +71,97 @@ abbreviation DecSetOf ::
    'BASIC_VALUE COMPOSITE_VALUE set" where
 "DecSetOf v \<equiv> DecSet (SetOf v)"
 
-subsection {* Sort Membership *}
-
-instantiation COMPOSITE_VALUE :: (BASIC_SORT) COMPOSITE_SORT
-begin
-definition MkInt_COMPOSITE_VALUE [simp] :
-"MkInt_COMPOSITE_VALUE i = BasicVal (MkInt i)"
-definition DestInt_COMPOSITE_VALUE [simp] :
-"DestInt_COMPOSITE_VALUE v = DestInt (ValOf v)"
-definition IsInt_COMPOSITE_VALUE [simp] :
-"IsInt_COMPOSITE_VALUE v \<longleftrightarrow> (IsBasicVal v) \<and> IsInt (ValOf v)"
-definition MkBool_COMPOSITE_VALUE [simp] :
-"MkBool_COMPOSITE_VALUE b = BasicVal (MkBool b)"
-definition DestBool_COMPOSITE_VALUE [simp] :
-"DestBool_COMPOSITE_VALUE v = DestBool (ValOf v)"
-definition IsBool_COMPOSITE_VALUE [simp] :
-"IsBool_COMPOSITE_VALUE v \<longleftrightarrow> (IsBasicVal v) \<and> IsBool (ValOf v)"
-definition MkStr_COMPOSITE_VALUE [simp] :
-"MkStr_COMPOSITE_VALUE s = BasicVal (MkStr s)"
-definition DestStr_COMPOSITE_VALUE [simp] :
-"DestStr_COMPOSITE_VALUE v = DestStr (ValOf v)"
-definition IsStr_COMPOSITE_VALUE [simp] :
-"IsStr_COMPOSITE_VALUE v \<longleftrightarrow> (IsBasicVal v) \<and> IsStr (ValOf v)"
-definition MkPair_COMPOSITE_VALUE [simp] :
-"MkPair_COMPOSITE_VALUE v1_v2 = (uncurry PairVal) v1_v2"
-definition DestPair_COMPOSITE_VALUE [simp] :
-"DestPair_COMPOSITE_VALUE v = PairOf v"
-definition IsPair_COMPOSITE_VALUE [simp] :
-"IsPair_COMPOSITE_VALUE v \<longleftrightarrow> IsPairVal v"
-definition MkSet_COMPOSITE_VALUE [simp] :
-"MkSet_COMPOSITE_VALUE vs = EncSetVal vs"
-definition DestSet_COMPOSITE_VALUE [simp] :
-"DestSet_COMPOSITE_VALUE v = DecSetOf v"
-definition IsSet_COMPOSITE_VALUE [simp] :
-"IsSet_COMPOSITE_VALUE v \<longleftrightarrow> IsSetVal v"
-instance
-apply (intro_classes)
-apply (simp_all add: uncurry_def)
-done
-end
-
-subsection {* Lifting Functors *}
+subsection {* Typing and Refinement *}
 
 fun lift_type_rel_composite ::
   "('BASIC_VALUE \<Rightarrow> 'BASIC_TYPE \<Rightarrow> bool) \<Rightarrow>
    ('BASIC_VALUE COMPOSITE_VALUE \<Rightarrow>
     'BASIC_TYPE COMPOSITE_TYPE \<Rightarrow> bool)"
-  ("(_ \<bowtie> _ :/ _)" [50, 51] 50) where
-"type_rel \<bowtie> (BasicVal v) : (BasicType t) = (type_rel v t)" |
-"type_rel \<bowtie> (BasicVal v) : (PairType t1 t2) = False" |
-"type_rel \<bowtie> (BasicVal v) : (SetType t) = False" |
-"type_rel \<bowtie> (PairVal v1 v2) : (BasicType t) = False" |
-"type_rel \<bowtie> (PairVal v1 v2) : (PairType t1 t2) =
- ((type_rel \<bowtie> v1 : t1) \<and> (type_rel \<bowtie> v2 : t2))" |
-"type_rel \<bowtie> (PairVal v1 v2) : (SetType t) = False" |
-"type_rel \<bowtie> (SetVal vs) : (BasicType t) = False" |
-"type_rel \<bowtie> (SetVal vs) : (PairType t1 t2) = False" |
-"type_rel \<bowtie> (SetVal vs) : (SetType t) =
- (\<forall> v \<in> DecSet(vs) . (type_rel) \<bowtie> v : t)"
+  ("(_ \<up> _ : _)" [50, 51] 50) where
+"type_rel \<up> (BasicVal v) : (BasicType t) = (type_rel v t)" |
+"type_rel \<up> (PairVal v1 v2) : (PairType t1 t2) =
+   ((type_rel \<up>  v1 : t1) \<and> (type_rel \<up>  v2 : t2))" |
+"type_rel \<up> (SetVal vs) : (SetType t) =
+   (\<forall> v \<in> DecSet(vs) . type_rel \<up>  v : t)" |
+"(type_rel \<up> _ : _) = False"
 
 fun lift_value_ref_composite ::
   "('BASIC_VALUE \<Rightarrow> 'BASIC_VALUE \<Rightarrow> bool) \<Rightarrow>
    ('BASIC_VALUE COMPOSITE_VALUE \<Rightarrow>
     'BASIC_VALUE COMPOSITE_VALUE \<Rightarrow> bool)"
-  ("(_ \<bowtie> _ \<sqsubseteq>/ _)" [50, 51] 50) where
-"value_ref \<bowtie> (BasicVal v) \<sqsubseteq> (BasicVal v') = (value_ref v v')" |
-"value_ref \<bowtie> (BasicVal v) \<sqsubseteq> (PairVal v1' v2') = False" |
-"value_ref \<bowtie> (BasicVal v) \<sqsubseteq> (SetVal vs') = False" |
-"value_ref \<bowtie> (PairVal v1 v2) \<sqsubseteq> (BasicVal v') = False" |
-"value_ref \<bowtie> (PairVal v1 v2) \<sqsubseteq> (PairVal v1' v2') = (v1 = v1' \<and> v2 = v2')" |
-"value_ref \<bowtie> (PairVal v1 v2) \<sqsubseteq> (SetVal vs') = False" |
-"value_ref \<bowtie> (SetVal vs) \<sqsubseteq> (BasicVal v') = False" |
-"value_ref \<bowtie> (SetVal vs) \<sqsubseteq> (PairVal v1' v2') = False" |
-"value_ref \<bowtie> (SetVal vs) \<sqsubseteq> (SetVal vs') = (vs = vs')"
+  ("(_ \<up> _ \<sqsubseteq>v/ _)" [50, 51] 50) where
+"value_ref \<up> (BasicVal v) \<sqsubseteq>v (BasicVal v') = (value_ref v v')" |
+"value_ref \<up> (PairVal v1 v2) \<sqsubseteq>v (PairVal v1' v2') =
+   (v1 = v1' \<and> v2 = v2')" |
+"value_ref \<up> (SetVal vs) \<sqsubseteq>v (SetVal vs') = (vs = vs')" |
+"(value_ref \<up> _ \<sqsubseteq>v _) = False"
+
+subsection {* Sort Membership *}
+
+instantiation COMPOSITE_VALUE :: (BASIC_SORT) COMPOSITE_SORT
+begin
+definition ValueRef_COMPOSITE_VALUE :
+"ValueRef_COMPOSITE_VALUE =
+ lift_value_ref_composite (VALUE_SORT_class.ValueRef)"
+definition MkInt_COMPOSITE_VALUE :
+"MkInt_COMPOSITE_VALUE i = BasicVal (MkInt i)"
+definition DestInt_COMPOSITE_VALUE :
+"DestInt_COMPOSITE_VALUE v = DestInt (BasicOf v)"
+definition IsInt_COMPOSITE_VALUE :
+"IsInt_COMPOSITE_VALUE v = ((IsBasicVal v) \<and> IsInt (BasicOf v))"
+definition MkBool_COMPOSITE_VALUE :
+"MkBool_COMPOSITE_VALUE b = BasicVal (MkBool b)"
+definition DestBool_COMPOSITE_VALUE :
+"DestBool_COMPOSITE_VALUE v = DestBool (BasicOf v)"
+definition IsBool_COMPOSITE_VALUE :
+"IsBool_COMPOSITE_VALUE v = ((IsBasicVal v) \<and> IsBool (BasicOf v))"
+definition MkStr_COMPOSITE_VALUE :
+"MkStr_COMPOSITE_VALUE s = BasicVal (MkStr s)"
+definition DestStr_COMPOSITE_VALUE :
+"DestStr_COMPOSITE_VALUE v = DestStr (BasicOf v)"
+definition IsStr_COMPOSITE_VALUE :
+"IsStr_COMPOSITE_VALUE v = ((IsBasicVal v) \<and> IsStr (BasicOf v))"
+definition MkPair_COMPOSITE_VALUE :
+"MkPair_COMPOSITE_VALUE v1_v2 = (uncurry PairVal) v1_v2"
+definition DestPair_COMPOSITE_VALUE :
+"DestPair_COMPOSITE_VALUE v = PairOf v"
+definition IsPair_COMPOSITE_VALUE :
+"IsPair_COMPOSITE_VALUE v = (IsPairVal v)"
+definition MkSet_COMPOSITE_VALUE :
+"MkSet_COMPOSITE_VALUE vs = EncSetVal vs"
+definition DestSet_COMPOSITE_VALUE :
+"DestSet_COMPOSITE_VALUE v = DecSetOf v"
+definition IsSet_COMPOSITE_VALUE :
+"IsSet_COMPOSITE_VALUE v = (IsSetVal v)"
+instance
+apply (intro_classes)
+done
+end
+
+subsubsection {* Default Simplifications *}
+
+declare ValueRef_COMPOSITE_VALUE [simp]
+declare MkInt_COMPOSITE_VALUE [simp]
+declare DestInt_COMPOSITE_VALUE [simp]
+declare IsInt_COMPOSITE_VALUE [simp]
+declare MkBool_COMPOSITE_VALUE [simp]
+declare DestBool_COMPOSITE_VALUE [simp]
+declare IsBool_COMPOSITE_VALUE [simp]
+declare MkStr_COMPOSITE_VALUE [simp]
+declare DestStr_COMPOSITE_VALUE [simp]
+declare IsStr_COMPOSITE_VALUE [simp]
+declare MkPair_COMPOSITE_VALUE [simp]
+declare DestPair_COMPOSITE_VALUE [simp]
+declare IsPair_COMPOSITE_VALUE [simp]
+declare MkSet_COMPOSITE_VALUE [simp]
+declare DestSet_COMPOSITE_VALUE [simp]
+declare IsSet_COMPOSITE_VALUE [simp]
 
 subsection {* Locale @{text "COMPOSITE_VALUE"} *}
 
-text {* I am not sure yet whether a locale is really necessary here. *}
-
 locale COMPOSITE_VALUE =
   VALUE "lift_type_rel_composite basic_type_rel"
-    "lift_value_ref_composite basic_value_ref"
-for basic_type_rel :: "'BASIC_VALUE :: BASIC_SORT \<Rightarrow> 'BASIC_TYPE \<Rightarrow> bool" and
-  basic_value_ref :: "'BASIC_VALUE :: BASIC_SORT \<Rightarrow> 'BASIC_VALUE \<Rightarrow> bool"
+for basic_type_rel :: "'BASIC_VALUE :: BASIC_SORT \<Rightarrow> 'BASIC_TYPE \<Rightarrow> bool"
 begin
 
 subsubsection {* Constructors *}
@@ -172,11 +177,6 @@ definition MkBool ::
 definition MkStr ::
   "string \<Rightarrow> 'BASIC_VALUE COMPOSITE_VALUE" where
 "MkStr = STRING_SORT_class.MkStr"
-
-definition MkVal ::
-  "'BASIC_VALUE \<Rightarrow>
-   'BASIC_VALUE COMPOSITE_VALUE" where
-"MkVal = BasicVal"
 
 definition MkPair ::
   "'BASIC_VALUE COMPOSITE_VALUE \<times>
@@ -203,11 +203,6 @@ definition DestStr ::
   "'BASIC_VALUE COMPOSITE_VALUE \<Rightarrow> string" where
 "DestStr = STRING_SORT_class.DestStr"
 
-definition DestVal ::
-  "'BASIC_VALUE COMPOSITE_VALUE \<Rightarrow>
-   'BASIC_VALUE" where
-"DestVal = ValOf"
-
 definition DestPair ::
   "'BASIC_VALUE COMPOSITE_VALUE \<Rightarrow>
   ('BASIC_VALUE COMPOSITE_VALUE \<times>
@@ -233,10 +228,6 @@ definition IsStr ::
   "'BASIC_VALUE COMPOSITE_VALUE \<Rightarrow> bool" where
 "IsStr = STRING_SORT_class.IsStr"
 
-definition IsVal ::
-  "'BASIC_VALUE COMPOSITE_VALUE \<Rightarrow> bool" where
-"IsVal = IsBasicVal"
-
 definition IsPair ::
   "'BASIC_VALUE COMPOSITE_VALUE \<Rightarrow> bool" where
 "IsPair = PAIR_SORT_class.IsPair"
@@ -245,26 +236,23 @@ definition IsSet ::
   "'BASIC_VALUE COMPOSITE_VALUE \<Rightarrow> bool" where
 "IsSet = SET_SORT_class.IsSet"
 
-subsubsection {* Default Simplificiations *}
+subsubsection {* Default Simplifications *}
 
 declare MkInt_def [simp]
 declare MkBool_def [simp]
 declare MkStr_def [simp]
-declare MkVal_def [simp]
 declare MkPair_def [simp]
 declare MkSet_def [simp]
 
 declare DestInt_def [simp]
 declare DestBool_def [simp]
 declare DestStr_def [simp]
-declare DestVal_def [simp]
 declare DestPair_def [simp]
 declare DestSet_def [simp]
 
 declare IsInt_def [simp]
 declare IsBool_def [simp]
 declare IsStr_def [simp]
-declare IsVal_def [simp]
 declare IsPair_def [simp]
 declare IsSet_def [simp]
 end
@@ -289,7 +277,7 @@ done
 
 text {* The following theorem facilitates locale instantiation. *}
 
-theorem TYPED_PRED_inst [intro!, simp] :
+theorem VALUE_COMPOSITE_VALUE_inst [intro!, simp] :
 "\<lbrakk>VALUE type_rel\<rbrakk> \<Longrightarrow> COMPOSITE_VALUE type_rel"
 apply (simp add: COMPOSITE_VALUE_def)
 apply (auto)
