theories/models/utp_default_value.thy
@@ -3,12 +3,12 @@
 (* Author: Frank Zeyda, University of York                                    *)
 (******************************************************************************)
 theory utp_default_value
-imports "../utp_common" "../utp_sorts" "../generic/utp_abstract_value"
+imports GLOBAL "../utp_common" "../utp_sorts" "../generic/utp_abstract_value"
 begin
 
 section {* Default Values *}
 
-subsection {* Data Types *}
+subsection {* Value Encoding *}
 
 datatype DEFAULT_VALUE =
   IntVal "int" |
@@ -20,7 +20,7 @@ datatype DEFAULT_TYPE =
   BoolType |
   StringType
 
-subsection {* Tests *}
+subsubsection {* Tests *}
 
 primrec IsIntVal :: "DEFAULT_VALUE \<Rightarrow> bool" where
 "IsIntVal (IntVal _) = True" |
@@ -37,10 +37,37 @@ primrec IsStringVal :: "DEFAULT_VALUE \<Rightarrow> bool" where
 "IsStringVal (BoolVal _) = False" |
 "IsStringVal (StringVal _) = True"
 
+subsection {* Typing and Refinement *}
+
+fun default_type_rel :: "DEFAULT_VALUE \<Rightarrow> DEFAULT_TYPE \<Rightarrow> bool"  where
+"default_type_rel (IntVal _) IntType = True" |
+"default_type_rel (IntVal _) BoolType = False" |
+"default_type_rel (IntVal _) StringType = False" |
+"default_type_rel (BoolVal _) IntType = False" |
+"default_type_rel (BoolVal _) BoolType = True" |
+"default_type_rel (BoolVal _) StringType = False" |
+"default_type_rel (StringVal _) IntType = False" |
+"default_type_rel (StringVal _) BoolType = False" |
+"default_type_rel (StringVal _) StringType = True"
+
+defs default_type_rel [simp] :
+"GLOBAL.type_rel \<equiv> default_type_rel"
+
+text {* The refinement ordering for basic values is flat. *}
+
+definition default_value_ref ::
+  "DEFAULT_VALUE \<Rightarrow> DEFAULT_VALUE \<Rightarrow> bool"  where
+"default_value_ref v1 v2 = (v1 = v2)"
+
+declare  default_value_ref_def [simp]
+
 subsection {* Sort Membership *}
 
 instantiation DEFAULT_VALUE :: BASIC_SORT
 begin
+definition ValueRef_DEFAULT_VALUE ::
+  "DEFAULT_VALUE \<Rightarrow> DEFAULT_VALUE \<Rightarrow> bool" where
+"ValueRef_DEFAULT_VALUE = default_value_ref"
 definition MkInt_DEFAULT_VALUE :: "int \<Rightarrow> DEFAULT_VALUE" where
 "MkInt_DEFAULT_VALUE i = IntVal i"
 primrec DestInt_DEFAULT_VALUE :: "DEFAULT_VALUE \<Rightarrow> int" where
@@ -57,39 +84,25 @@ definition MkStr_DEFAULT_VALUE :: "string \<Rightarrow> DEFAULT_VALUE" where
 "MkStr_DEFAULT_VALUE s = StringVal s"
 primrec DestStr_DEFAULT_VALUE:: "DEFAULT_VALUE \<Rightarrow> string" where
 "DestStr_DEFAULT_VALUE (StringVal s) = s"
-definition IsString_DEFAULT_VALUE :: "DEFAULT_VALUE \<Rightarrow> bool" where
-"IsString_DEFAULT_VALUE = IsStringVal"
+definition IsStr_DEFAULT_VALUE :: "DEFAULT_VALUE \<Rightarrow> bool" where
+"IsStr_DEFAULT_VALUE = IsStringVal"
 instance
 apply (intro_classes)
-apply (simp add: MkBool_DEFAULT_VALUE_def DestBool_DEFAULT_VALUE_def)
-apply (simp add: MkInt_DEFAULT_VALUE_def DestInt_DEFAULT_VALUE_def)
-apply (simp add: MkStr_DEFAULT_VALUE_def DestStr_DEFAULT_VALUE_def)
 done
 end
 
-subsection {* Typing and Refinement *}
+subsubsection {* Default Simplifications *}
 
-fun default_type_rel ::
-  "DEFAULT_VALUE \<Rightarrow> DEFAULT_TYPE \<Rightarrow> bool" (infix ":" 50) where
-"(IntVal _) : IntType = True" |
-"(IntVal _) : BoolType = False" |
-"(IntVal _) : StringType = False" |
-"(BoolVal _) : IntType = False" |
-"(BoolVal _) : BoolType = True" |
-"(BoolVal _) : StringType = False" |
-"(StringVal _) : IntType = False" |
-"(StringVal _) : BoolType = False" |
-"(StringVal _) : StringType = True"
-
-no_notation default_type_rel (infix ":" 50)
-
-text {* The refinement order of default values is flat. *}
-
-definition default_value_ref ::
-  "DEFAULT_VALUE \<Rightarrow> DEFAULT_VALUE \<Rightarrow> bool"  (infix "\<sqsubseteq>v" 50) where
-"v1 \<sqsubseteq>v v2 \<longleftrightarrow> (v1 = v2)"
-
-no_notation default_type_rel (infix "\<sqsubseteq>v" 50)
+declare ValueRef_DEFAULT_VALUE_def [simp]
+declare MkInt_DEFAULT_VALUE_def [simp]
+declare DestInt_DEFAULT_VALUE_def [simp]
+declare IsInt_DEFAULT_VALUE_def [simp]
+declare MkBool_DEFAULT_VALUE_def [simp]
+declare DestBool_DEFAULT_VALUE_def [simp]
+declare IsBool_DEFAULT_VALUE_def [simp]
+declare MkStr_DEFAULT_VALUE_def [simp]
+declare DestStr_DEFAULT_VALUE_def [simp]
+declare IsStr_DEFAULT_VALUE_def [simp]
 
 subsection {* Theorems *}
 
@@ -102,6 +115,20 @@ apply (auto)
 apply (rule_tac x = "BoolVal b" in exI)
 apply (auto)
 apply (rule_tac x = "StringVal s" in exI)
+apply (auto)
+done
+
+subsection {* Proof Experiments *}
+
+theorem "(IntVal 1) : IntType"
+apply (auto)
+done
+
+theorem "(IntVal 1) \<sqsubseteq>v (IntVal 1)"
+apply (auto)
+done
+
+theorem "((MkInt 1) :: DEFAULT_VALUE) : IntType"
 apply (auto)
 done
 end
