theories/models/utp_ho1_value.thy
@@ -3,12 +3,14 @@
 (* Author: Frank Zeyda, University of York                                    *)
 (******************************************************************************)
 theory utp_ho1_value
-imports "../GLOBAL" "../utp_sorts" utp_std_pred
+imports "../GLOBAL" "../utp_sorts" "../generic/utp_composite_value"
+  utp_default_value
+  utp_std_pred
 begin
 
 section {* HO1 Values *}
 
-subsection {* Program Values *}
+subsection {* Program Encoding *}
 
 typedef STD_PREDICATE = STD_PREDICATE
 apply (rule_tac x = "FALSE" in exI)
@@ -20,106 +22,7 @@ apply (rule_tac x = "{}" in exI)
 apply (auto)
 done
 
-subsection {* Data Types *}
-
-types PROG_VALUE = STD_PREDICATE
-
-datatype HO1_VALUE =
-  IntVal "int" |
-  BoolVal "bool" |
-  StringVal "string" |
-  ProgVal "PROG_VALUE"
-
-types PROG_TYPE = STD_ALPHABET
-
-datatype HO1_TYPE =
-  IntType |
-  BoolType |
-  StringType |
-  ProgType "PROG_TYPE"
-
-subsection {* Constructors *}
-
-definition MkProg :: "PROG_VALUE \<Rightarrow> HO1_VALUE" where
-"MkProg = ProgVal"
-
-subsection {* Destructors *}
-
-primrec DestProg :: "HO1_VALUE \<Rightarrow> PROG_VALUE" where
-"DestProg (ProgVal p) = p"
-
-subsection {* Tests *}
-
-primrec IsIntVal :: "HO1_VALUE \<Rightarrow> bool" where
-"IsIntVal (IntVal _) = True" |
-"IsIntVal (BoolVal _) = False" |
-"IsIntVal (StringVal _) = False" |
-"IsIntVal (ProgVal _) = False"
-
-primrec IsBoolVal :: "HO1_VALUE \<Rightarrow> bool" where
-"IsBoolVal (IntVal _) = False" |
-"IsBoolVal (BoolVal _) = True" |
-"IsBoolVal (StringVal _) = False" |
-"IsBoolVal (ProgVal _) = False"
-
-primrec IsStringVal :: "HO1_VALUE \<Rightarrow> bool" where
-"IsStringVal (IntVal _) = False" |
-"IsStringVal (BoolVal _) = False" |
-"IsStringVal (StringVal _) = True" |
-"IsStringVal (ProgVal _) = False"
-
-primrec IsProgVal :: "HO1_VALUE \<Rightarrow> bool" where
-"IsProgVal (IntVal _) = False" |
-"IsProgVal (BoolVal _) = False" |
-"IsProgVal (StringVal _) = False" |
-"IsProgVal (ProgVal _) = True"
-
-subsection {* Sort Membership *}
-
-instantiation HO1_VALUE :: BASIC_SORT
-begin
-definition MkInt_HO1_VALUE :: "int \<Rightarrow> HO1_VALUE" where
-"MkInt_HO1_VALUE i = IntVal i"
-primrec DestInt_HO1_VALUE :: "HO1_VALUE \<Rightarrow> int" where
-"DestInt_HO1_VALUE (IntVal i) = i"
-definition IsInt_HO1_VALUE :: "HO1_VALUE \<Rightarrow> bool" where
-"IsInt_HO1_VALUE = IsIntVal"
-definition MkBool_HO1_VALUE :: "bool \<Rightarrow> HO1_VALUE" where
-"MkBool_HO1_VALUE b = BoolVal b"
-primrec DestBool_HO1_VALUE :: "HO1_VALUE \<Rightarrow> bool" where
-"DestBool_HO1_VALUE (BoolVal b) = b"
-definition IsBool_HO1_VALUE :: "HO1_VALUE \<Rightarrow> bool" where
-"IsBool_HO1_VALUE = IsBoolVal"
-definition MkStr_HO1_VALUE :: "string \<Rightarrow> HO1_VALUE" where
-"MkStr_HO1_VALUE s = StringVal s"
-primrec DestStr_HO1_VALUE :: "HO1_VALUE \<Rightarrow> string" where
-"DestStr_HO1_VALUE (StringVal s) = s"
-definition IsStr_HO1_VALUE :: "HO1_VALUE \<Rightarrow> bool" where
-"IsStr_HO1_VALUE = IsStringVal"
-instance
-apply (intro_classes)
-apply (simp add: MkBool_HO1_VALUE_def DestBool_HO1_VALUE_def)
-apply (simp add: MkInt_HO1_VALUE_def DestInt_HO1_VALUE_def)
-apply (simp add: MkStr_HO1_VALUE_def DestStr_HO1_VALUE_def)
-done
-end
-
-subsection {* Typing and Refinement *}
-
-fun ho1_type_rel :: "HO1_VALUE \<Rightarrow> HO1_TYPE \<Rightarrow> bool" where
-"ho1_type_rel (IntVal _) IntType = True" |
-"ho1_type_rel (BoolVal _) BoolType = True" |
-"ho1_type_rel (StringVal _) StringType = True" |
-"ho1_type_rel (ProgVal p) (ProgType a) =
- (\<alpha> (Rep_STD_PREDICATE p) = (Rep_STD_ALPHABET a))" |
-"ho1_type_rel _ _ = False"
-
-fun ho1_value_ref :: "HO1_VALUE \<Rightarrow> HO1_VALUE \<Rightarrow> bool" where
-"ho1_value_ref (ProgVal p1) (ProgVal p2) =
- ((Rep_STD_PREDICATE p1) \<sqsubseteq>v (Rep_STD_PREDICATE p2))" |
-"ho1_value_ref v1 v2 = (v1 = v2)"
-
-subsection {* Default Simplifications *}
+subsubsection {* Default Simplifications *}
 
 declare Abs_STD_PREDICATE_inverse [simp]
 declare Rep_STD_PREDICATE_inverse [simp]
@@ -133,17 +36,228 @@ declare Abs_STD_ALPHABET_inject [simp, intro!]
 declare Rep_STD_ALPHABET_inject [simp, intro!]
 declare Rep_STD_ALPHABET [simp]
 
+subsection {* Value Encoding *}
+
+types BASE_VALUE = "STD_VALUE"
+types PROG_VALUE = "STD_PREDICATE"
+
+datatype HO1_VALUE =
+  BaseVal "BASE_VALUE" |
+  ProgVal "PROG_VALUE"
+
+types BASE_TYPE = "STD_TYPE"
+types PROG_TYPE = "STD_ALPHABET"
+
+datatype HO1_TYPE =
+  BaseType "BASE_TYPE" |
+  ProgType "PROG_TYPE"
+
+subsubsection {* Destructors *}
+
+primrec BaseOf :: "HO1_VALUE \<Rightarrow> BASE_VALUE" where
+"BaseOf (BaseVal v) = v"
+
+primrec ProgOf :: "HO1_VALUE \<Rightarrow> PROG_VALUE" where
+"ProgOf (ProgVal p) = p"
+
+subsubsection {* Tests *}
+
+primrec IsBaseVal :: "HO1_VALUE \<Rightarrow> bool" where
+"IsBaseVal (BaseVal _) = True" |
+"IsBaseVal (ProgVal _) = False"
+
+primrec IsProgVal :: "HO1_VALUE \<Rightarrow> bool" where
+"IsProgVal (BaseVal _) = False" |
+"IsProgVal (ProgVal _) = True"
+
+subsection {* Typing and Refinement *}
+
+definition std_prog_type_rel :: "PROG_VALUE \<Rightarrow> PROG_TYPE \<Rightarrow> bool" where
+"std_prog_type_rel p a = (\<alpha> (Rep_STD_PREDICATE p) = (Rep_STD_ALPHABET a))"
+
+definition std_prog_value_ref :: "PROG_VALUE \<Rightarrow> PROG_VALUE \<Rightarrow> bool" where
+"std_prog_value_ref p1 p2 = ((Rep_STD_PREDICATE p1) \<sqsubseteq> (Rep_STD_PREDICATE p2))"
+
+defs global_std_prog_type_rel [simp] :
+"GLOBAL.type_rel \<equiv> std_prog_type_rel"
+
+fun ho1_type_rel :: "HO1_VALUE \<Rightarrow> HO1_TYPE \<Rightarrow> bool" where
+"ho1_type_rel (BaseVal v) (BaseType t) = (v : t)" |
+"ho1_type_rel (BaseVal v) (ProgType t) = False" |
+"ho1_type_rel (ProgVal v) (ProgType t) = (std_prog_type_rel v t)" |
+"ho1_type_rel (ProgVal v) (BaseType t) = False"
+
+fun ho1_value_ref :: "HO1_VALUE \<Rightarrow> HO1_VALUE \<Rightarrow> bool" where
+"ho1_value_ref (BaseVal v1) (BaseVal v2) = (v1 \<sqsubseteq>v v2)" |
+"ho1_value_ref (BaseVal v1) (ProgVal v2) = False" |
+"ho1_value_ref (ProgVal v1) (ProgVal v2) = (std_prog_value_ref v1 v2)" |
+"ho1_value_ref (ProgVal v1) (BaseVal v2) = False"
+
+declare std_prog_type_rel_def [simp]
+declare std_prog_value_ref_def [simp]
+
+subsection {* Sort Membership *}
+
+instantiation STD_PREDICATE :: VALUE_SORT
+begin
+definition ValueRef_STD_PREDICATE [simp] :
+"ValueRef_STD_PREDICATE = std_prog_value_ref"
+instance
+apply (intro_classes)
+done
+end
+
+text {*
+  Instantiation to @{text "COMPOSITE_SORT"} succeeds because we removed the
+  inverse assumptions from the various value sorts; in particular, previous
+  attempts failed to establish the inverse assumptions for pairs and sets.
+*}
+
+instantiation HO1_VALUE :: COMPOSITE_SORT
+begin
+definition ValueRef_HO1_VALUE [simp] :
+"ValueRef_HO1_VALUE = ho1_value_ref"
+definition MkInt_HO1_VALUE [simp] :
+"MkInt_HO1_VALUE i = BaseVal (MkInt i)"
+definition DestInt_HO1_VALUE [simp] :
+"DestInt_HO1_VALUE v = DestInt (BaseOf v)"
+definition IsInt_HO1_VALUE [simp] :
+"IsInt_HO1_VALUE v = ((IsBaseVal v) \<and> (IsInt (BaseOf v)))"
+definition MkBool_HO1_VALUE [simp] :
+"MkBool_HO1_VALUE i = BaseVal (MkBool i)"
+definition DestBool_HO1_VALUE [simp] :
+"DestBool_HO1_VALUE v = DestBool (BaseOf v)"
+definition IsBool_HO1_VALUE [simp] :
+"IsBool_HO1_VALUE v = ((IsBaseVal v) \<and> IsBool (BaseOf v))"
+definition MkStr_HO1_VALUE [simp] :
+"MkStr_HO1_VALUE i = BaseVal (MkStr i)"
+definition DestStr_HO1_VALUE [simp] :
+"DestStr_HO1_VALUE v = DestStr (BaseOf v)"
+definition IsStr_HO1_VALUE [simp] :
+"IsStr_HO1_VALUE v = ((IsBaseVal v) \<and> IsStr (BaseOf v))"
+definition MkPair_HO1_VALUE [simp] :
+"MkPair_HO1_VALUE v1_v2 =
+   BaseVal (MkPair (BaseOf (fst v1_v2), BaseOf (snd v1_v2)))"
+definition DestPair_HO1_VALUE [simp] :
+"DestPair_HO1_VALUE v = (
+   BaseVal (fst (DestPair (BaseOf v))),
+   BaseVal (snd (DestPair (BaseOf v))))"
+definition IsPair_HO1_VALUE [simp] :
+"IsPair_HO1_VALUE v = ((IsBaseVal v) \<and> IsPair (BaseOf v))"
+definition MkSet_HO1_VALUE [simp] :
+"MkSet_HO1_VALUE vs = BaseVal (MkSet (BaseOf ` vs))"
+definition DestSet_HO1_VALUE [simp] :
+"DestSet_HO1_VALUE v = BaseVal ` (DestSet (BaseOf v))"
+definition IsSet_HO1_VALUE [simp] :
+"IsSet_HO1_VALUE v = ((IsBaseVal v) \<and> IsSet (BaseOf v))"
+instance
+apply (intro_classes)
+done
+end
+
+subsection {* Locale @{text "HO1_VALUE"} *}
+
+locale HO1_VALUE_LOCALE = VALUE "ho1_type_rel"
+begin
+
+subsubsection {* Constructors *}
+
+definition MkInt :: "int \<Rightarrow> HO1_VALUE" where
+"MkInt = INT_SORT_class.MkInt"
+
+definition MkBool :: "bool \<Rightarrow> HO1_VALUE" where
+"MkBool = BOOL_SORT_class.MkBool"
+
+definition MkStr :: "string \<Rightarrow> HO1_VALUE" where
+"MkStr = STRING_SORT_class.MkStr"
+
+definition MkPair ::
+  "(HO1_VALUE \<times> HO1_VALUE) \<Rightarrow> HO1_VALUE" where
+"MkPair = PAIR_SORT_class.MkPair"
+
+definition MkSet :: "HO1_VALUE set \<Rightarrow> HO1_VALUE" where
+"MkSet = SET_SORT_class.MkSet"
+
+definition MkProg :
+"MkProg p = ProgVal (Abs_STD_PREDICATE p)"
+
+subsubsection {* Destructors *}
+
+definition DestInt :: "HO1_VALUE \<Rightarrow> int" where
+"DestInt = INT_SORT_class.DestInt"
+
+definition DestBool :: "HO1_VALUE \<Rightarrow> bool" where
+"DestBool = BOOL_SORT_class.DestBool"
+
+definition DestStr :: "HO1_VALUE \<Rightarrow> string" where
+"DestStr = STRING_SORT_class.DestStr"
+
+definition DestPair ::
+  "HO1_VALUE \<Rightarrow> (HO1_VALUE \<times> HO1_VALUE)" where
+"DestPair = PAIR_SORT_class.DestPair"
+
+definition DestSet :: "HO1_VALUE \<Rightarrow> HO1_VALUE set" where
+"DestSet = SET_SORT_class.DestSet"
+
+definition DestProg :
+"DestProg v = Rep_STD_PREDICATE (ProgOf v)"
+
+subsubsection {* Tests *}
+
+definition IsInt :: "HO1_VALUE \<Rightarrow> bool" where
+"IsInt = INT_SORT_class.IsInt"
+
+definition IsBool :: "HO1_VALUE \<Rightarrow> bool" where
+"IsBool = BOOL_SORT_class.IsBool"
+
+definition IsStr :: "HO1_VALUE \<Rightarrow> bool" where
+"IsStr = STRING_SORT_class.IsStr"
+
+definition IsPair :: "HO1_VALUE \<Rightarrow> bool" where
+"IsPair = PAIR_SORT_class.IsPair"
+
+definition IsSet :: "HO1_VALUE \<Rightarrow> bool" where
+"IsSet = SET_SORT_class.IsSet"
+
+definition IsProg :: "HO1_VALUE \<Rightarrow> bool" where
+"IsProg = IsProgVal"
+
+subsubsection {* Default Simplifications *}
+
+declare MkInt_def [simp]
+declare MkBool_def [simp]
+declare MkStr_def [simp]
+declare MkPair_def [simp]
+declare MkSet_def [simp]
+declare MkProg [simp]
+
+declare DestInt_def [simp]
+declare DestBool_def [simp]
+declare DestStr_def [simp]
+declare DestPair_def [simp]
+declare DestSet_def [simp]
+declare DestProg [simp]
+
+declare IsInt_def [simp]
+declare IsBool_def [simp]
+declare IsStr_def [simp]
+declare IsPair_def [simp]
+declare IsSet_def [simp]
+declare IsProg_def [simp]
+end
+
 subsection {* Theorems *}
 
 theorem VALUE_ho1_type_rel [simp] :
 "VALUE ho1_type_rel"
 apply (unfold_locales)
 apply (induct_tac t)
-apply (rule_tac x = "IntVal i" in exI)
-apply (auto)
-apply (rule_tac x = "BoolVal b" in exI)
-apply (auto)
-apply (rule_tac x = "StringVal s" in exI)
+apply (subgoal_tac "COMPOSITE_VALUE default_type_rel")
+apply (simp add: COMPOSITE_VALUE_def VALUE_def)
+apply (drule_tac x = "COMPOSITE_TYPE" in spec)
+apply (safe)
+apply (rule_tac x = "BaseVal x" in exI)
+apply (simp)
 apply (auto)
 apply (rule_tac x =
   "ProgVal (Abs_STD_PREDICATE
