theories/models/utp_ho2_value.thy
@@ -3,12 +3,14 @@
 (* Author: Frank Zeyda, University of York                                    *)
 (******************************************************************************)
 theory utp_ho2_value
-imports "../GLOBAL" "../utp_sorts" utp_ho1_pred
+imports "../GLOBAL" "../utp_sorts" "../generic/utp_composite_value"
+  utp_ho1_value
+  utp_ho1_pred
 begin
 
 section {* HO2 Values *}
 
-subsection {* Program Values *}
+subsection {* Program Encoding *}
 
 typedef HO1_PREDICATE = HO1_PREDICATE
 apply (rule_tac x = "FALSE" in exI)
@@ -20,131 +22,7 @@ apply (rule_tac x = "{}" in exI)
 apply (auto)
 done
 
-subsection {* Data Types *}
-
-types PROG1_VALUE = STD_PREDICATE
-types PROG2_VALUE = HO1_PREDICATE
-
-datatype HO2_VALUE =
-  IntVal "int" |
-  BoolVal "bool" |
-  StringVal "string" |
-  Prog1Val "PROG1_VALUE" |
-  Prog2Val "PROG2_VALUE"
-
-types PROG1_TYPE = STD_ALPHABET
-types PROG2_TYPE = HO1_ALPHABET
-
-datatype HO2_TYPE =
-  IntType |
-  BoolType |
-  StringType |
-  Prog1Type "PROG1_TYPE" |
-  Prog2Type "PROG2_TYPE"
-
-subsection {* Constructors *}
-
-definition MkProg1 :: "PROG1_VALUE \<Rightarrow> HO2_VALUE" where
-"MkProg1 = Prog1Val"
-
-definition MkProg2 :: "PROG2_VALUE \<Rightarrow> HO2_VALUE" where
-"MkProg2 = Prog2Val"
-
-subsection {* Destructors *}
-
-primrec DestProg1 :: "HO2_VALUE \<Rightarrow> PROG1_VALUE" where
-"DestProg1 (Prog1Val p) = p"
-
-primrec DestProg2 :: "HO2_VALUE \<Rightarrow> PROG2_VALUE" where
-"DestProg2 (Prog2Val p) = p"
-
-subsection {* Tests *}
-
-primrec IsIntVal :: "HO2_VALUE \<Rightarrow> bool" where
-"IsIntVal (IntVal _) = True" |
-"IsIntVal (BoolVal _) = False" |
-"IsIntVal (StringVal _) = False" |
-"IsIntVal (Prog1Val _) = False" |
-"IsIntVal (Prog2Val _) = False"
-
-primrec IsBoolVal :: "HO2_VALUE \<Rightarrow> bool" where
-"IsBoolVal (IntVal _) = False" |
-"IsBoolVal (BoolVal _) = True" |
-"IsBoolVal (StringVal _) = False" |
-"IsBoolVal (Prog1Val _) = False" |
-"IsBoolVal (Prog2Val _) = False"
-
-primrec IsStringVal :: "HO2_VALUE \<Rightarrow> bool" where
-"IsStringVal (IntVal _) = False" |
-"IsStringVal (BoolVal _) = False" |
-"IsStringVal (StringVal _) = True" |
-"IsStringVal (Prog1Val _) = False" |
-"IsStringVal (Prog2Val _) = False"
-
-primrec IsProg1Val :: "HO2_VALUE \<Rightarrow> bool" where
-"IsProg1Val (IntVal _) = False" |
-"IsProg1Val (BoolVal _) = False" |
-"IsProg1Val (StringVal _) = False" |
-"IsProg1Val (Prog1Val _) = True" |
-"IsProg1Val (Prog2Val _) = False"
-
-primrec IsProg2Val :: "HO2_VALUE \<Rightarrow> bool" where
-"IsProg2Val (IntVal _) = False" |
-"IsProg2Val (BoolVal _) = False" |
-"IsProg2Val (StringVal _) = False" |
-"IsProg2Val (Prog1Val _) = False" |
-"IsProg2Val (Prog2Val _) = True"
-
-subsection {* Sort Membership *}
-
-instantiation HO2_VALUE :: BASIC_SORT
-begin
-definition MkInt_HO2_VALUE :: "int \<Rightarrow> HO2_VALUE" where
-"MkInt_HO2_VALUE i = IntVal i"
-primrec DestInt_HO2_VALUE :: "HO2_VALUE \<Rightarrow> int" where
-"DestInt_HO2_VALUE (IntVal i) = i"
-definition IsInt_HO2_VALUE :: "HO2_VALUE \<Rightarrow> bool" where
-"IsInt_HO2_VALUE = IsIntVal"
-definition MkBool_HO2_VALUE :: "bool \<Rightarrow> HO2_VALUE" where
-"MkBool_HO2_VALUE b = BoolVal b"
-primrec DestBool_HO2_VALUE :: "HO2_VALUE \<Rightarrow> bool" where
-"DestBool_HO2_VALUE (BoolVal b) = b"
-definition IsBool_HO2_VALUE :: "HO2_VALUE \<Rightarrow> bool" where
-"IsBool_HO2_VALUE = IsBoolVal"
-definition MkStr_HO2_VALUE :: "string \<Rightarrow> HO2_VALUE" where
-"MkStr_HO2_VALUE s = StringVal s"
-primrec DestStr_HO2_VALUE :: "HO2_VALUE \<Rightarrow> string" where
-"DestStr_HO2_VALUE (StringVal s) = s"
-definition IsStr_HO2_VALUE :: "HO2_VALUE \<Rightarrow> bool" where
-"IsStr_HO2_VALUE = IsStringVal"
-instance
-apply (intro_classes)
-apply (simp add: MkBool_HO2_VALUE_def DestBool_HO2_VALUE_def)
-apply (simp add: MkInt_HO2_VALUE_def DestInt_HO2_VALUE_def)
-apply (simp add: MkStr_HO2_VALUE_def DestStr_HO2_VALUE_def)
-done
-end
-
-subsection {* Typing and Refinement *}
-
-fun ho2_type_rel :: "HO2_VALUE \<Rightarrow> HO2_TYPE \<Rightarrow> bool" where
-"ho2_type_rel (IntVal _) IntType = True" |
-"ho2_type_rel (BoolVal _) BoolType = True" |
-"ho2_type_rel (StringVal _) StringType = True" |
-"ho2_type_rel (Prog1Val p) (Prog1Type a) =
- (\<alpha> (Rep_STD_PREDICATE p) = (Rep_STD_ALPHABET a))" |
-"ho2_type_rel (Prog2Val p) (Prog2Type a) =
- (\<alpha> (Rep_HO1_PREDICATE p) = (Rep_HO1_ALPHABET a))" |
-"ho2_type_rel _ _ = False"
-
-fun ho2_value_ref :: "HO2_VALUE \<Rightarrow> HO2_VALUE \<Rightarrow> bool" where
-"ho2_value_ref (Prog1Val p1) (Prog1Val p2) =
- ((Rep_STD_PREDICATE p1) \<sqsubseteq>v (Rep_STD_PREDICATE p2))" |
-"ho2_value_ref (Prog2Val p1) (Prog2Val p2) =
- ((Rep_HO1_PREDICATE p1) \<sqsubseteq>v (Rep_HO1_PREDICATE p2))" |
-"ho2_value_ref v1 v2 = (v1 = v2)"
-subsection {* Default Simplifications *}
-subsection {* Default Simplifications *}
+subsubsection {* Default Simplifications *}
 
 declare Abs_HO1_PREDICATE_inverse [simp]
 declare Rep_HO1_PREDICATE_inverse [simp]
@@ -158,21 +36,269 @@ declare Abs_HO1_ALPHABET_inject [simp, intro!]
 declare Rep_HO1_ALPHABET_inject [simp, intro!]
 declare Rep_HO1_ALPHABET [simp]
 
+subsection {* Value Encoding *}
+
+types BASE_VALUE = "STD_VALUE"
+types PROG1_VALUE = "STD_PREDICATE"
+types PROG2_VALUE = "HO1_PREDICATE"
+
+datatype HO2_VALUE =
+  BaseVal "BASE_VALUE" |
+  Prog1Val "PROG1_VALUE" |
+  Prog2Val "PROG2_VALUE"
+
+types BASE_TYPE = "STD_TYPE"
+types PROG1_TYPE = "STD_ALPHABET"
+types PROG2_TYPE = "HO1_ALPHABET"
+
+datatype HO2_TYPE =
+  BaseType "BASE_TYPE" |
+  Prog1Type "PROG1_TYPE" |
+  Prog2Type "PROG2_TYPE"
+
+subsubsection {* Destructors *}
+
+primrec BaseOf :: "HO2_VALUE \<Rightarrow> BASE_VALUE" where
+"BaseOf (BaseVal v) = v"
+
+primrec Prog1Of :: "HO2_VALUE \<Rightarrow> PROG1_VALUE" where
+"Prog1Of (Prog1Val p) = p"
+
+primrec Prog2Of :: "HO2_VALUE \<Rightarrow> PROG2_VALUE" where
+"Prog2Of (Prog2Val p) = p"
+
+subsubsection {* Tests *}
+
+primrec IsBaseVal :: "HO2_VALUE \<Rightarrow> bool" where
+"IsBaseVal (BaseVal _) = True" |
+"IsBaseVal (Prog1Val _) = False" |
+"IsBaseVal (Prog2Val _) = False"
+
+primrec IsProg1Val :: "HO2_VALUE \<Rightarrow> bool" where
+"IsProg1Val (BaseVal _) = False" |
+"IsProg1Val (Prog1Val _) = True" |
+"IsProg1Val (Prog2Val _) = False"
+
+primrec IsProg2Val :: "HO2_VALUE \<Rightarrow> bool" where
+"IsProg2Val (BaseVal _) = False" |
+"IsProg2Val (Prog1Val _) = False" |
+"IsProg2Val (Prog2Val _) = True"
+
+subsection {* Typing and Refinement *}
+
+definition ho1_prog_type_rel :: "PROG2_VALUE \<Rightarrow> PROG2_TYPE \<Rightarrow> bool" where
+"ho1_prog_type_rel p a = (\<alpha> (Rep_HO1_PREDICATE p) = (Rep_HO1_ALPHABET a))"
+
+definition ho1_prog_value_ref :: "PROG2_VALUE \<Rightarrow> PROG2_VALUE \<Rightarrow> bool" where
+"ho1_prog_value_ref p1 p2 = ((Rep_HO1_PREDICATE p1) \<sqsubseteq> (Rep_HO1_PREDICATE p2))"
+
+defs global_ho1_prog_type_rel [simp] :
+"GLOBAL.type_rel \<equiv> ho1_prog_type_rel"
+
+fun ho2_type_rel :: "HO2_VALUE \<Rightarrow> HO2_TYPE \<Rightarrow> bool" where
+"ho2_type_rel (BaseVal v) (BaseType t) = (v : t)" |
+"ho2_type_rel (BaseVal v) (Prog1Type t) = False" |
+"ho2_type_rel (BaseVal v) (Prog2Type t) = False" |
+"ho2_type_rel (Prog1Val v) (BaseType t) = False" |
+"ho2_type_rel (Prog1Val v) (Prog1Type t) = (std_prog_type_rel v t)" |
+"ho2_type_rel (Prog1Val v) (Prog2Type t) = False" |
+"ho2_type_rel (Prog2Val v) (BaseType t) = False" |
+"ho2_type_rel (Prog2Val v) (Prog1Type t) = False" |
+"ho2_type_rel (Prog2Val v) (Prog2Type t) = (ho1_prog_type_rel v t)"
+
+fun ho2_value_ref :: "HO2_VALUE \<Rightarrow> HO2_VALUE \<Rightarrow> bool" where
+"ho2_value_ref (BaseVal v1) (BaseVal v2) = (v1 \<sqsubseteq>v v2)" |
+"ho2_value_ref (BaseVal v1) (Prog1Val v2) = False" |
+"ho2_value_ref (BaseVal v1) (Prog2Val v2) = False" |
+"ho2_value_ref (Prog1Val v1) (BaseVal v2) = False" |
+"ho2_value_ref (Prog1Val v1) (Prog1Val v2) = (std_prog_value_ref v1 v2)" |
+"ho2_value_ref (Prog1Val v1) (Prog2Val v2) = False" |
+"ho2_value_ref (Prog2Val v1) (BaseVal v2) = False" |
+"ho2_value_ref (Prog2Val v1) (Prog1Val v2) = False" |
+"ho2_value_ref (Prog2Val v1) (Prog2Val v2) = (ho1_prog_value_ref v1 v2)"
+
+declare ho1_prog_type_rel_def [simp]
+declare ho1_prog_value_ref_def [simp]
+
+subsection {* Sort Membership *}
+
+instantiation HO1_PREDICATE :: VALUE_SORT
+begin
+definition ValueRef_HO1_PREDICATE [simp] :
+"ValueRef_HO1_PREDICATE = ho1_prog_value_ref"
+instance
+apply (intro_classes)
+done
+end
+
+text {*
+  Instantiation to @{text "COMPOSITE_SORT"} succeeds because we removed the
+  inverse assumptions from the various value sorts; in particular, previous
+  attempts failed to establish the inverse assumptions for pairs and sets.
+*}
+
+instantiation HO2_VALUE :: COMPOSITE_SORT
+begin
+definition ValueRef_HO2_VALUE [simp] :
+"ValueRef_HO2_VALUE = ho2_value_ref"
+definition MkInt_HO2_VALUE [simp] :
+"MkInt_HO2_VALUE i = BaseVal (MkInt i)"
+definition DestInt_HO2_VALUE [simp] :
+"DestInt_HO2_VALUE v = DestInt (BaseOf v)"
+definition IsInt_HO2_VALUE [simp] :
+"IsInt_HO2_VALUE v = ((IsBaseVal v) \<and> (IsInt (BaseOf v)))"
+definition MkBool_HO2_VALUE [simp] :
+"MkBool_HO2_VALUE i = BaseVal (MkBool i)"
+definition DestBool_HO2_VALUE [simp] :
+"DestBool_HO2_VALUE v = DestBool (BaseOf v)"
+definition IsBool_HO2_VALUE [simp] :
+"IsBool_HO2_VALUE v = ((IsBaseVal v) \<and> IsBool (BaseOf v))"
+definition MkStr_HO2_VALUE [simp] :
+"MkStr_HO2_VALUE i = BaseVal (MkStr i)"
+definition DestStr_HO2_VALUE [simp] :
+"DestStr_HO2_VALUE v = DestStr (BaseOf v)"
+definition IsStr_HO2_VALUE [simp] :
+"IsStr_HO2_VALUE v = ((IsBaseVal v) \<and> IsStr (BaseOf v))"
+definition MkPair_HO2_VALUE [simp] :
+"MkPair_HO2_VALUE v1_v2 =
+   BaseVal (MkPair (BaseOf (fst v1_v2), BaseOf (snd v1_v2)))"
+definition DestPair_HO2_VALUE [simp] :
+"DestPair_HO2_VALUE v = (
+   BaseVal (fst (DestPair (BaseOf v))),
+   BaseVal (snd (DestPair (BaseOf v))))"
+definition IsPair_HO2_VALUE [simp] :
+"IsPair_HO2_VALUE v = ((IsBaseVal v) \<and> IsPair (BaseOf v))"
+definition MkSet_HO2_VALUE [simp] :
+"MkSet_HO2_VALUE vs = BaseVal (MkSet (BaseOf ` vs))"
+definition DestSet_HO2_VALUE [simp] :
+"DestSet_HO2_VALUE v = BaseVal ` (DestSet (BaseOf v))"
+definition IsSet_HO2_VALUE [simp] :
+"IsSet_HO2_VALUE v = ((IsBaseVal v) \<and> IsSet (BaseOf v))"
+instance
+apply (intro_classes)
+done
+end
+
+subsection {* Locale @{text "HO2_VALUE"} *}
+
+locale HO2_VALUE_LOCALE = VALUE "ho2_type_rel"
+begin
+
+subsubsection {* Constructors *}
+
+definition MkInt :: "int \<Rightarrow> HO2_VALUE" where
+"MkInt = INT_SORT_class.MkInt"
+
+definition MkBool :: "bool \<Rightarrow> HO2_VALUE" where
+"MkBool = BOOL_SORT_class.MkBool"
+
+definition MkStr :: "string \<Rightarrow> HO2_VALUE" where
+"MkStr = STRING_SORT_class.MkStr"
+
+definition MkPair ::
+  "(HO2_VALUE \<times> HO2_VALUE) \<Rightarrow> HO2_VALUE" where
+"MkPair = PAIR_SORT_class.MkPair"
+
+definition MkSet :: "HO2_VALUE set \<Rightarrow> HO2_VALUE" where
+"MkSet = SET_SORT_class.MkSet"
+
+definition MkProg1 :
+"MkProg1 p = Prog1Val (Abs_STD_PREDICATE p)"
+
+definition MkProg2 :
+"MkProg2 p = Prog2Val (Abs_HO1_PREDICATE p)"
+
+subsubsection {* Destructors *}
+
+definition DestInt :: "HO2_VALUE \<Rightarrow> int" where
+"DestInt = INT_SORT_class.DestInt"
+
+definition DestBool :: "HO2_VALUE \<Rightarrow> bool" where
+"DestBool = BOOL_SORT_class.DestBool"
+
+definition DestStr :: "HO2_VALUE \<Rightarrow> string" where
+"DestStr = STRING_SORT_class.DestStr"
+
+definition DestPair ::
+  "HO2_VALUE \<Rightarrow> (HO2_VALUE \<times> HO2_VALUE)" where
+"DestPair = PAIR_SORT_class.DestPair"
+
+definition DestSet :: "HO2_VALUE \<Rightarrow> HO2_VALUE set" where
+"DestSet = SET_SORT_class.DestSet"
+
+definition DestProg1 :
+"DestProg1 v = Rep_STD_PREDICATE (Prog1Of v)"
+
+definition DestProg2 :
+"DestProg2 v = Rep_HO1_PREDICATE (Prog2Of v)"
+
+subsubsection {* Tests *}
+
+definition IsInt :: "HO2_VALUE \<Rightarrow> bool" where
+"IsInt = INT_SORT_class.IsInt"
+
+definition IsBool :: "HO2_VALUE \<Rightarrow> bool" where
+"IsBool = BOOL_SORT_class.IsBool"
+
+definition IsStr :: "HO2_VALUE \<Rightarrow> bool" where
+"IsStr = STRING_SORT_class.IsStr"
+
+definition IsPair :: "HO2_VALUE \<Rightarrow> bool" where
+"IsPair = PAIR_SORT_class.IsPair"
+
+definition IsSet :: "HO2_VALUE \<Rightarrow> bool" where
+"IsSet = SET_SORT_class.IsSet"
+
+definition IsProg1 :: "HO2_VALUE \<Rightarrow> bool" where
+"IsProg1 = IsProg1Val"
+
+definition IsProg2 :: "HO2_VALUE \<Rightarrow> bool" where
+"IsProg2 = IsProg2Val"
+
+subsubsection {* Default Simplifications *}
+
+declare MkInt_def [simp]
+declare MkBool_def [simp]
+declare MkStr_def [simp]
+declare MkPair_def [simp]
+declare MkSet_def [simp]
+declare MkProg1 [simp]
+declare MkProg2 [simp]
+
+declare DestInt_def [simp]
+declare DestBool_def [simp]
+declare DestStr_def [simp]
+declare DestPair_def [simp]
+declare DestSet_def [simp]
+declare DestProg1 [simp]
+declare DestProg2 [simp]
+
+declare IsInt_def [simp]
+declare IsBool_def [simp]
+declare IsStr_def [simp]
+declare IsPair_def [simp]
+declare IsSet_def [simp]
+declare IsProg1_def [simp]
+declare IsProg2_def [simp]
+end
+
 subsection {* Theorems *}
 
 theorem VALUE_ho2_type_rel [simp] :
 "VALUE ho2_type_rel"
 apply (unfold_locales)
 apply (induct_tac t)
-apply (rule_tac x = "IntVal i" in exI)
-apply (auto)
-apply (rule_tac x = "BoolVal b" in exI)
-apply (auto)
-apply (rule_tac x = "StringVal s" in exI)
+(* TODO: Fix the remainder of the proof! *)
+apply (subgoal_tac "COMPOSITE_VALUE default_type_rel")
+apply (simp add: COMPOSITE_VALUE_def VALUE_def)
+apply (drule_tac x = "COMPOSITE_TYPE" in spec)
+apply (safe)
+apply (rule_tac x = "BaseVal x" in exI)
+apply (simp)
 apply (auto)
 apply (rule_tac x =
   "Prog1Val (Abs_STD_PREDICATE
-    (STD.FalseP (Rep_STD_ALPHABET STD_ALPHABET)))" in exI)
+     (STD.FalseP (Rep_STD_ALPHABET STD_ALPHABET)))" in exI)
 apply (simp)
 apply (subgoal_tac "Rep_STD_ALPHABET STD_ALPHABET \<in> STD.WF_ALPHABET")
 apply (subst Abs_STD_PREDICATE_inverse)
