theories/generic/utp_binding_fun.thy
@@ -8,7 +8,7 @@ begin
 
 section {* Binding Functions *}
 
-text {* TODO: Develop a proof tactic for membership to @{text "WF_BINDING_FUN"}. *}
+text {* TODO: Develop a tactic for membership to @{text "WF_BINDING_FUN"}. *}
 
 context GEN_PRED
 begin
@@ -21,35 +21,35 @@ theorem binding_fun_non_interfere1 :
 "\<lbrakk>x \<in> a\<rbrakk> \<Longrightarrow>
  (\<lambda> b . f (b x)) \<in> WF_BINDING_FUN a"
 apply (simp add: WF_BINDING_FUN_def)
-apply (simp add: BINDING_EQUIV_def)
+apply (simp add: binding_equiv_def)
 done
 
 theorem binding_fun_non_interfere2 :
 "\<lbrakk>x1 \<in> a; x2 \<in> a\<rbrakk> \<Longrightarrow>
  (\<lambda> b . f (b x1) (b x2)) \<in> WF_BINDING_FUN a"
 apply (simp add: WF_BINDING_FUN_def)
-apply (simp add: BINDING_EQUIV_def)
+apply (simp add: binding_equiv_def)
 done
 
 theorem binding_fun_non_interfere3 :
 "\<lbrakk>x1 \<in> a; x2 \<in> a; x3 \<in> a\<rbrakk> \<Longrightarrow>
  (\<lambda> b . f (b x1) (b x2) (b x3)) \<in> WF_BINDING_FUN a"
 apply (simp add: WF_BINDING_FUN_def)
-apply (simp add: BINDING_EQUIV_def)
+apply (simp add: binding_equiv_def)
 done
 
 theorem binding_fun_non_interfere4 :
 "\<lbrakk>x1 \<in> a; x2 \<in> a; x3 \<in> a; x4 \<in> a\<rbrakk> \<Longrightarrow>
  (\<lambda> b . f (b x1) (b x2) (b x3) (b x4)) \<in> WF_BINDING_FUN a"
 apply (simp add: WF_BINDING_FUN_def)
-apply (simp add: BINDING_EQUIV_def)
+apply (simp add: binding_equiv_def)
 done
 
 theorem binding_fun_non_interfere5 :
 "\<lbrakk>x1 \<in> a; x2 \<in> a; x3 \<in> a; x4 \<in> a; x5 \<in> a\<rbrakk> \<Longrightarrow>
  (\<lambda> b . f (b x1) (b x2) (b x3) (b x4) (b x5)) \<in> WF_BINDING_FUN a"
 apply (simp add: WF_BINDING_FUN_def)
-apply (simp add: BINDING_EQUIV_def)
+apply (simp add: binding_equiv_def)
 done
 
 (* Maybe the following are actually not needed in practice. *)
