theories/generic/utp_function.thy
@@ -8,19 +8,18 @@ begin
 
 section {* Functions on Predicates *}
 
+types ('VALUE, 'TYPE) ALPHA_FUNCTION =
+  "('VALUE, 'TYPE) ALPHA_PREDICATE \<Rightarrow>
+   ('VALUE, 'TYPE) ALPHA_PREDICATE"
+
 context GEN_PRED
 begin
-
-types ('a, 'b) ALPHA_FUNCTION =
-  "('a, 'b) ALPHA_PREDICATE \<Rightarrow>
-   ('a, 'b) ALPHA_PREDICATE"
-
-definition WF_ALPHA_FUNCTION :: "('TYPE VAR, 'VALUE) ALPHA_FUNCTION set" where
+definition WF_ALPHA_FUNCTION :: "('VALUE, 'TYPE) ALPHA_FUNCTION set" where
 "WF_ALPHA_FUNCTION =
  {f . \<forall> p \<in> WF_ALPHA_PREDICATE . f p \<in> WF_ALPHA_PREDICATE}"
 
 definition WF_ALPHA_FUNCTION_OVER ::
-  "'TYPE VAR ALPHABET \<Rightarrow> ('TYPE VAR, 'VALUE) ALPHA_FUNCTION set" where
+  "'TYPE ALPHABET \<Rightarrow> ('VALUE, 'TYPE) ALPHA_FUNCTION set" where
 "\<lbrakk>a \<in> WF_ALPHABET\<rbrakk> \<Longrightarrow>
  WF_ALPHA_FUNCTION_OVER a =
  {f . \<forall> p \<in> WF_ALPHA_PREDICATE_OVER a . f p \<in> WF_ALPHA_PREDICATE}"
@@ -28,8 +27,8 @@ definition WF_ALPHA_FUNCTION_OVER ::
 text {* The following could be useful, this still needs to be explored! *}
 
 definition WF_ALPHA_FUNCTION_BETWEEN ::
-  "['TYPE VAR ALPHABET, 'TYPE VAR ALPHABET] \<Rightarrow>
-   ('TYPE VAR, 'VALUE) ALPHA_FUNCTION set" where
+  "['TYPE ALPHABET, 'TYPE ALPHABET] \<Rightarrow>
+   ('VALUE, 'TYPE) ALPHA_FUNCTION set" where
 "\<lbrakk>a1 \<in> WF_ALPHABET;
  a2 \<in> WF_ALPHABET\<rbrakk> \<Longrightarrow>
  WF_ALPHA_FUNCTION_BETWEEN a1 a2 \<equiv>
@@ -37,15 +36,15 @@ definition WF_ALPHA_FUNCTION_BETWEEN ::
 
 section {* Restrictions *}
 
-definition IDEMPOTENT :: "('TYPE VAR, 'VALUE) ALPHA_FUNCTION set" where
+definition IDEMPOTENT :: "('VALUE, 'TYPE) ALPHA_FUNCTION set" where
 "IDEMPOTENT = {f . \<forall> p \<in> WF_ALPHA_PREDICATE . f (f p) = f p}"
 
 definition IDEMPOTENT_OVER ::
-  "'TYPE VAR ALPHABET \<Rightarrow> ('TYPE VAR, 'VALUE) ALPHA_FUNCTION set" where
+  "'TYPE ALPHABET \<Rightarrow> ('VALUE, 'TYPE) ALPHA_FUNCTION set" where
 "\<lbrakk>a \<in> WF_ALPHABET\<rbrakk> \<Longrightarrow>
  IDEMPOTENT_OVER a = {f . \<forall> p \<in> WF_ALPHA_PREDICATE_OVER a . f (f p) = f p}"
 
-definition MONOTONIC :: "('TYPE VAR, 'VALUE) ALPHA_FUNCTION set" where
+definition MONOTONIC :: "('VALUE, 'TYPE) ALPHA_FUNCTION set" where
 "MONOTONIC =
  {f \<in> WF_ALPHA_FUNCTION .
    \<forall> a \<in> WF_ALPHABET .
@@ -53,7 +52,7 @@ definition MONOTONIC :: "('TYPE VAR, 'VALUE) ALPHA_FUNCTION set" where
    \<forall> p2 \<in> WF_ALPHA_PREDICATE_OVER a . p1 \<sqsubseteq> p2 \<longrightarrow> f(p1) \<sqsubseteq> f(p2)}"
 
 definition MONOTONIC_OVER ::
-  "'TYPE VAR ALPHABET \<Rightarrow> ('TYPE VAR, 'VALUE) ALPHA_FUNCTION set" where
+  "'TYPE ALPHABET \<Rightarrow> ('VALUE, 'TYPE) ALPHA_FUNCTION set" where
 "\<lbrakk>a \<in> WF_ALPHABET\<rbrakk> \<Longrightarrow>
  MONOTONIC_OVER a =
  {f \<in> WF_ALPHA_FUNCTION_OVER a .
