theories/models/utp_models.thy
@@ -1,14 +1,14 @@
 (******************************************************************************)
-(* Title: utp/theories/utp_models.thy                                         *)
+(* Title: utp/models/utp_models.thy                                           *)
 (* Author: Frank Zeyda, University of York                                    *)
 (******************************************************************************)
-theory utp_theories
+theory utp_models
 imports
   utp_default_value
   utp_std_pred
   utp_ho1_value
-  utp_ho2_value
   utp_ho1_pred
+  utp_ho2_value
   utp_ho2_pred
 begin
 
