theories/utp_types.thy
@@ -1,0 +1,31 @@
+(******************************************************************************)
+(* Title: utp/utp_types.thy                                                   *)
+(* Author: Frank Zeyda, University of York                                    *)
+(******************************************************************************)
+theory utp_types
+imports utp_common "generic/utp_name"
+begin
+
+section {* Type Synonyms *}
+
+types 'TYPE VAR = "NAME \<times> 'TYPE"
+
+types 'TYPE ALPHABET =
+  "('TYPE VAR) set"
+
+types ('VALUE, 'TYPE) BINDING =
+  "('TYPE VAR) \<Rightarrow> 'VALUE"
+
+types ('VALUE, 'TYPE) BINDING_SET =
+  "('VALUE, 'TYPE) BINDING set"
+
+types ('VALUE, 'TYPE) BINDING_FUN =
+  "('VALUE, 'TYPE) BINDING \<Rightarrow> bool"
+
+types ('VALUE, 'TYPE) ALPHA_PREDICATE =
+  "('TYPE ALPHABET) \<times> ('VALUE, 'TYPE) BINDING set"
+
+types ('VALUE, 'TYPE) ALPHA_FUNCTION =
+  "('VALUE, 'TYPE) ALPHA_PREDICATE \<Rightarrow>
+   ('VALUE, 'TYPE) ALPHA_PREDICATE"
+end
